extraction/ExtractPulseGPU.fst
@@ -136,34 +136,14 @@ let gpu_translate_expr : translate_expr_t = fun env e ->
     EBufWrite (cb r, cb idx, cb v)
 
   | MLE_App ({ expr = MLE_Name p }, [
-        _pre;
-        _post;
-        { expr = MLE_Fun (_, body) }
-      ])
-    when string_of_mlpath p = "GPU.Base.launch_kernel_1" ->
-    let hd, args = head_and_args body in
-    let kcall : mlexpr = with_ty ml_unit_ty <| MLE_Name ([], "PULSE_KCALL") in
-    (* Filter out unit arguments. Not great, not sure why they remain *)
-    let args' = List.filter (fun a -> match a.expr with
-                                    | MLE_Const MLC_Unit -> false
-                                    | _ -> true) args in
-    let e' =
-      with_ty ml_unit_ty <|
-        MLE_App (kcall, [ hd;
-                          with_ty ml_int_ty <| MLE_Const (MLC_Int ("1", Some (Unsigned, FStar.Const.Int32)));
-                          with_ty ml_int_ty <| MLE_Const (MLC_Int ("1", Some (Unsigned, FStar.Const.Int32))) ]
-                        @ args')
-    in
-    cb e'
-
-  | MLE_App ({ expr = MLE_Name p }, [
         _uid;
+        nblk;
         nthr;
         _pre;
         _post;
         { expr = MLE_Fun (_, body) }
       ])
-    when string_of_mlpath p = "GPU.Base.launch_kernel_n" ->
+    when string_of_mlpath p = "GPU.Kernel.kernel_n_as_n_m" ->
     let hd, args = head_and_args body in
     (* Filter out unit arguments. Not great, not sure why they remain *)
     let args' = List.filter (fun a -> match a.expr with
@@ -173,8 +153,8 @@ let gpu_translate_expr : translate_expr_t = fun env e ->
     let e' =
       with_ty ml_unit_ty <|
         MLE_App (kcall, [ hd;
-                          nthr;
-                          with_ty ml_int_ty <| MLE_Const (MLC_Int ("1", Some (Unsigned, FStar.Const.Int32))) ]
+                          nblk;
+                          nthr ]
                         @ args')
     in
     cb e'
