src/lib/GPU.Kernel.fsti
@@ -1,0 +1,124 @@
+module GPU.Kernel
+
+open Pulse.Lib.Pervasives
+open FStar.Tactics.V2
+open FStar.Seq
+open Pulse.Lib.BigStar
+open GPU.SizeT
+open GPU.Array
+open GPU.Base
+open GPU.MatrixBarrier
+open FStar.Mul
+module U32 = FStar.UInt32
+
+(* f<<<nblk, nthr>>>(...); *)
+```pulse
+val
+fn launch_kernel_n_m_sync
+  (#u1: int)
+  (nblk : U32.t { 0 < nblk /\ nblk <= max_blocks })
+  (nthr : U32.t { 0 < nthr /\ nthr <= max_threads })
+  (#pre #post : (tid:nat{ 0 <= tid /\ tid < (nblk * nthr) } -> slprop))
+
+  (barrier : (it:nat -> from: nat { 0 <= from /\ from < nthr } -> to: nat { 0 <= to /\ to < nthr } -> slprop))
+  (smem_sz : U32.t)
+  (smem : (to: nat { 0 <= to /\ to < nthr } -> slprop))
+  (smem_split :
+    (ar: gpu_array U32.t smem_sz) -> (v: FStar.Seq.seq U32.t) ->
+    stt_ghost unit emp_inames
+      (gpu_pts_to_array #U32.t #smem_sz ar #1.0R v) (fun _ -> bigstar 0 nthr smem))
+
+  (k :
+    (b : erased (GPU.Barrier2.barrier nthr)) -> (etid: erased tid_t { gdim_x etid == nblk /\ bdim_x etid == nthr }) ->
+    stt unit (         gpu ** thread_id etid ** smem (tidx_x etid) ** mbarrier_tok barrier b 0 (tidx_x etid) ** pre (thread_index etid))
+             (fun _ -> gpu ** thread_id etid ** smem (tidx_x etid) ** mbarrier_tok barrier b 0 (tidx_x etid) ** post (thread_index etid))
+  )
+  requires cpu ** bigstar #u1 0 (nblk * nthr) pre
+  ensures  cpu ** bigstar #u1 0 (nblk * nthr) post
+```
+
+(* f<<<nblk, nthr>>>(...); *)
+```pulse
+val
+fn launch_kernel_n_m
+  (#u1: int)
+  (nblk : U32.t { 0 < nblk /\ nblk <= max_blocks })
+  (nthr : U32.t { 0 < nthr /\ nthr <= max_threads })
+  (#pre #post : (tid:nat{ 0 <= tid /\ tid < (nblk * nthr) } -> slprop))
+  (k :
+    (etid: erased tid_t { gdim_x etid == nblk /\ bdim_x etid == nthr }) ->
+    stt unit (         gpu ** thread_id etid ** pre (thread_index etid))
+             (fun _ -> gpu ** thread_id etid ** post (thread_index etid))
+  )
+  requires cpu ** bigstar #u1 0 (nblk * nthr) pre
+  ensures  cpu ** bigstar #u1 0 (nblk * nthr) post
+```
+
+(* f<<<nblk, 1>>>(...); *)
+```pulse
+// Private
+fn kernel_n_as_n_m
+  (nblk  : U32.t { 0 < nblk /\ nblk <= max_blocks })
+  (#pre #post : (tid:nat{ 0 <= tid /\ tid < U32.v nblk } -> slprop))
+  (k :
+    (etid:erased tid_t { gdim_x etid == nblk /\ bdim_x etid == 1ul }) ->
+    stt unit (gpu ** thread_id etid ** pre (thread_index etid))
+             (fun _ -> gpu ** thread_id etid ** post (thread_index etid))
+  )
+  (etid:erased tid_t { gdim_x etid == nblk /\ bdim_x etid == 1ul })
+  requires gpu ** thread_id etid ** pre (thread_index etid)
+  ensures  gpu ** thread_id etid ** post (thread_index etid)
+{
+  k etid;
+}
+```
+
+```pulse
+fn launch_kernel_n
+  (#u1: int)
+  (nblk  : U32.t { 0 < nblk /\ nblk <= max_blocks })
+  (#pre #post : (tid:nat{ 0 <= tid /\ tid < U32.v nblk } -> slprop))
+  (k :
+    (etid:erased tid_t { gdim_x etid == nblk /\ bdim_x etid == 1ul }) ->
+    stt unit (gpu ** thread_id etid ** pre (thread_index etid))
+             (fun _ -> gpu ** thread_id etid ** post (thread_index etid))
+  )
+  requires cpu ** bigstar #u1 0 (U32.v nblk) pre
+  ensures  cpu ** bigstar #u1 0 (U32.v nblk) post
+{
+  rewrite (bigstar #u1 0 (U32.v nblk) pre) as (bigstar #u1 0 (U32.v nblk * 1) pre);
+  launch_kernel_n_m #u1 nblk 1ul #pre #post (fun etid -> kernel_n_as_n_m nblk #pre #post k etid);
+  rewrite (bigstar #u1 0 (U32.v nblk * 1) post) as (bigstar #u1 0 (U32.v nblk) post);
+}
+```
+
+(* f<<<1, 1>>>(...); *)
+```pulse
+// Private
+fn kernel_1_as_n
+  (#pre #post : slprop)
+  (k : unit ->
+    stt unit (gpu ** pre) (fun _ -> gpu ** post)
+  )
+  (etid:erased tid_t { gdim_x etid == 1ul /\ bdim_x etid == 1ul })
+  requires gpu ** thread_id etid ** pre
+  ensures  gpu ** thread_id etid ** post
+{
+  k ()
+}
+```
+
+```pulse
+fn launch_kernel_1
+  (#pre #post : slprop)
+  (k : unit ->
+    stt unit (gpu ** pre) (fun _ -> gpu ** post)
+  )
+  requires cpu ** pre
+  ensures  cpu ** post
+{
+  bigstar_single_intro 0 0 (fun (i: nat { 0 <= i /\ i < 1 }) -> pre);
+  launch_kernel_n 1ul (fun etid -> kernel_1_as_n #pre #post k etid);
+  bigstar_single_elim #0;
+}
+```
