src/lib/GPU.fsti
@@ -4,6 +4,7 @@ include GPU.Base
 include GPU.Ref
 include GPU.Types
 include GPU.Array
+include GPU.Kernel
 include GPU.SizeT
 include GPU.Barrier2
 include GPU.MatrixBarrier
